

$$2.a) Q_{n+1}(a) = Q_n(a) + \alpha [R_{n+1} - Q_n(a)]$$

$$Q_{n+1}(a) = Q_n(a)(1-\alpha) + \alpha R_{n+1}$$

$$\text{let } Q_n(a) \equiv x_n \quad R_n \equiv y_n$$

$$\therefore x_{n+1} = (1-\alpha)x_n + \alpha y_{n+1}$$

$$= (1-\alpha)((1-\alpha)x_{n-1} + \alpha y_n) + \alpha y_{n+1}$$

$$= (1-\alpha)^2 x_{n-1} + \alpha(y_{n+1} + (1-\alpha)y_n)$$

$$= (1-\alpha)^{n+1} x_0 + \alpha(y_{n+1} + \dots + (1-\alpha)^n y_1)$$

$\left[\begin{array}{l} \text{(note } (1-\alpha)^2 x_{n-1} \text{)} \\ \downarrow \\ (1-\alpha)^{n+1} x_0 \end{array} \right]$
 $\begin{array}{l} n-1+2=n+1 \\ n+1+0=n+1 \end{array}$

$$x_0 = 0$$

$$x_{n+1} = \alpha \sum_{i=0}^n (1-\alpha)^{n-i} y_{i+1} \Rightarrow Q_{n+1}(a) = \alpha \sum_{i=0}^n (1-\alpha)^{n-i} R_{i+1}$$

$$2b) Q_{n+1}(a) = \alpha [R_{n+1} + (1-\alpha)R_n + (1-\alpha)^2 R_{n-1} + \dots]$$

$$= \alpha R_{n+1} + \alpha(1-\alpha)R_n + \alpha(1-\alpha)^2 R_{n-1} + \dots$$

$\uparrow \quad \alpha > \alpha(1-\alpha) > \alpha(1-\alpha)^2 > \dots$

\therefore more weights on recent rewards

Since the distribution changes with time, we rely on put more weightage on recent happenings, thus tracking ~~going along with~~ change of environment with time.

$$2c) \alpha_n = \frac{\log(n+2)}{(n+2)} \quad \text{R-M algo :-}$$

$$1) \boxed{\alpha_n > 0} \quad \left[\begin{array}{l} \log(n+2) > 0 \text{ as } n \gg 1 \therefore n+2 > 3 \\ \therefore \log(n+2) > \log 3 > 0 \text{ [monotonic inc.]} \\ \Rightarrow \log(n+2)/(n+2) > 0 \end{array} \right]$$

$$2) \boxed{\sum \alpha_n = \infty} \quad (\text{To show})$$

$$S_k = \sum_{n=1}^k \frac{\log(n+2)}{(n+2)}$$

$$k=1 \Rightarrow S_1 = \frac{\log 3}{3}$$

$$k=2 \Rightarrow S_2 = \frac{\log 3}{3} + \frac{\log 4}{4}$$

$$\therefore S = \frac{\log 3}{3} + \frac{\log 4}{4} + \frac{\log 5}{5} + \dots$$

~~By integral test~~ let $f(x) = \frac{\log(x+2)}{(x+2)^2}$

$$\int_1^{\infty} f(x) dx = \int_3^{\infty} \frac{\log y}{y^2} dy = \left[-\frac{1}{y} (\log y) + \frac{1}{y} \right]_3^{\infty} = \frac{(\log 3)^2 - (\log 3)}{2}$$

$$t \rightarrow \infty, \int_1^t f(x) dx \rightarrow \infty$$

Since integral diverges, hence, $\sum_{n=1}^{\infty} f(n)$ also diverges.

[By integral test] [$f(x)$ is monotone decreasing as —

$$\text{let } f_1(x) = \frac{\log x}{x} \Rightarrow f_1'(x) = \frac{x \cdot \frac{1}{x} - (\log x) \cdot 1}{x^2} = \frac{1 - \log x}{x^2}$$

$$f_1'(x) = 0 \Rightarrow \log x = 1 \text{ or } \boxed{x = e}$$

$$\text{No. } f_1''(x) = \frac{d}{dx} \left(\frac{1}{x^2} - \frac{\log x}{x^2} \right) = \frac{-2}{x^3} - \frac{x \cdot \frac{1}{x^2} - 2 \log x}{x^4}$$

$$= -\frac{2}{x^3} - \frac{1}{x^3} + \frac{2 \log x}{x^3}$$

$$= -\frac{3 + 2 \log x}{x^3} \Big|_{x=e} < 0$$

hence $x = e$ maxima.

Thus after $x > e$ we

have the fn as ~~increasing~~ decreasing.

2) monotone decreasing

$$f_1'(x) = \frac{1 - \log x}{x^2} < 0 \Rightarrow \log x > 1 \Rightarrow x > e$$

hence, after $x > e$ we have monotonic decreasing.

~~Why~~ why $x > e$ satisfies $f(x)$?

$$f(x) = \frac{\log(x+2)}{(x+2)} \quad x > 1$$

$3 > e$. Hence, $f(x)$ satisfies properties of $f_1(x)$ for $x > 3 > e$.
So, $f(x)$ diverges.

(iii) $\sum a_n^2 < \infty$

$$f_1(x) = \frac{(\log x)^2}{x^2} \quad \int_1^{\infty} f_1(x) dx = \int_1^{\infty} \frac{(\log x)^2}{x^2} dx = \int_1^{\infty} \frac{1}{x} (\log x)^2 d(\log x)$$

$$= \boxed{\frac{1}{x} \int (\log x)^2 d(\log x)}$$

$$= (\log x)^2 \cdot \int \frac{dx}{x^2} - 2 \int (\log x) \left(\int \frac{dx}{x^2} \right) dx$$

$$= (\log x)^2 \frac{x^{-1}}{-1} + 2 \int \frac{\log x}{x} \cdot \frac{1}{x} dx = -\frac{(\log x)^2}{x} + 2 \int \frac{\log x}{x^2} dx$$

$$= -\frac{(\log x)^2}{x} + 2 \frac{\log x (-1)}{x} + 2 \int \frac{1}{x} \cdot \frac{1}{x} dx$$

$$= -\frac{(\log x)^2}{x} - 2 \frac{\log x}{x} - \frac{2}{x} = -\left[\frac{(\log x)^2 + 2 \log x + 2}{x} \right]$$

$$\therefore \int_1^{\infty} f_1(x) dx = - \left[\frac{(\log x)^2 + 2 \log x + 2}{x} \right]_1^{\infty} = - (0 - 2) = 2$$

$$\left[\lim_{x \rightarrow \infty} \frac{(\log x)^2 + 2 \log x + 2}{x} = \left(\frac{\infty}{\infty} \right) = \lim_{x \rightarrow \infty} \frac{2 \log x \cdot \frac{1}{x} + 2 \cdot \frac{1}{x}}{1} \right.$$

$$= \lim_{x \rightarrow \infty} \frac{2 \log x}{x} + \frac{2}{x} \rightarrow 0$$

$$\left. = \lim_{x \rightarrow \infty} \frac{2 \log x}{x} \left(\frac{\infty}{\infty} \right) = 2 \lim_{x \rightarrow \infty} \frac{1}{x} = 0 \right]$$

By integral test, $\sum_{n=1}^{\infty} \frac{\log(n+2)}{(n+2)^2}$ converges. (monotonic decreasing \rightarrow apparent).